Updating `AheadOf` to only allow gaps between thread pools when there aren't any writes in the log.

fullImpliesPartial.v
@@ -1,4 +1,4 @@
-Require Export stepPreservesRewind.  
+Require Export partialImpliesFull.  
 
 
 (*
@@ -10,7 +10,7 @@ Theorem replayInvalid : forall b1 b2 H H' rv wv tid e0 L e L' e' chkpnt HI,
                           validate tid rv wv e0 L H (abort chkpnt HI) ->
                           validate tid rv wv e0 L' H (abort chkpnt HI).
 Proof.
-  intros. dependent induction H0; auto.
+  intros. genDeps{{chkpnt; HI}}. dependent induction H0; intros; auto.
   dependent destruction H0; eauto. 
   {eapply IHreplay; eauto. eapply readPropAbort; eauto.
    constructor. }
@@ -18,93 +18,9 @@ Proof.
    constructor. }
   {eapply IHreplay; eauto. eapply readPropAbort; eauto.
    dependent destruction H4; constructor. }
-  {dependent destruction H2.
-   {admit. }
-   {admit. }
-  }
 Admitted. 
 
-  
 (*
-(*
- * If we can replay from one state to another and the first state is
- * invalid, then the second one must be too
- *)
-Theorem replayInvalid : forall H S e0 L e L' e' S' eA LA, 
-                          replay H (Some(S,e0),L,e) (Some(S,e0),L',e') ->
-                          validate S L H S' (abort eA LA) ->
-                          exists eA' LA', validate S L' H S' (abort eA' LA').
-Proof.
-  intros. dependent induction H0; eauto. 
-  {inv H0; eauto. 
-   {assert(validate S (readItem l E v::L) H S' (abort eA LA)).
-    eapply validateAbortPropogate; eauto. eapply IHreplay in H0; eauto. }
-   {assert(validate S (readItem l E v::L) H S' (abort eA LA)).
-    eapply validateAbortPropogate; eauto. eapply IHreplay in H0; eauto. }
-   {assert(validate S (writeItem l v::L) H S' (abort eA LA)).
-    eapply validateAbortPropogate; eauto. eapply IHreplay in H0; eauto. }
-  }
-Qed. 
-
-(*
- * If we can rewind/replay from one state to another and the final state is invalid,
- * then it must also be possible to rewind/replay to the portion that is still
- * valid as determined by validate 
- *)         
-Theorem rewindValidPortion : forall S L H S' e' L' e0 e, 
-                               rewind H (Some(S,e0),nil,e0) (Some(S,e0),L,e) ->
-                               validate S L H S' (abort e' L') ->
-                               rewind H (Some(S,e0),nil,e0) (Some(S,e0),L',e').
-Proof.
-  intros. dependent induction H0. 
-  {inv H1. }
-  {inv H1; eauto. 
-   {inv H2. 
-    {eapply IHrewind; eauto. }
-    {lookupSame. omega. }
-   }
-   {inv H2. 
-    {eapply IHrewind; eauto. }
-    {eapply decomposeEq in H10. subst. auto. }
-   }
-   {inv H2. eauto. }
-  }
-Qed. 
-
-(**
- * AheadOf holds under an extended heap if everything in the extension has a 
- * timestamp greater tan the transactions read version
- *)
-Theorem AheadOfExtension : forall H H' S t e0 L e C, 
-                      AheadOf H t (Some(S,e0),L,e) -> S < C ->
-                      Forall (fun x : location * term * stamp => getStamp x = C) H' ->
-                      AheadOf (H'++H) t (Some(S,e0),L,e).
-Proof.
-  intros. inv H0. 
-  econstructor. eapply replayHeapExtension; eauto.  
-Qed. 
-
-(*generalize to thread pools*)
-Theorem poolAheadOfExtension : forall H H' T1 T2 C,
-                    poolAheadOf H T1 T2 -> 
-                    Forall (fun x : location * term * stamp => getStamp x = C) H' ->
-                    poolRewind C H T2 ->
-                    poolAheadOf (H'++H) T1 T2.
-Proof.
-  intros. induction H0. 
-  {constructor. inv H2. 
-   {inv H0. constructor. }
-   {eapply AheadOfExtension; eauto. }
-  }
-  {inv H2. constructor; auto. } 
-Qed. 
-
-(*
-Ltac invertEq :=
-  match goal with
-      |H:?x = ?y |- _ => solve[inv H]
-  end. 
-*)
 
 (*if the beginning of a replay aborts, then so does the endpoint*)
 Theorem abortReplay : forall S L H C L' e' e'' L'' e e0, 
@@ -119,9 +35,11 @@ Qed.
 
 Inductive AheadOf (H : heap) : pool -> pool -> Prop :=
 | aheadOfNoTX : forall tid e, AheadOf H (Single(noTXThread tid e)) (Single(noTXThread tid e))
-| aheadOfTX : forall tid rv b b' e0 L L' e e' H',
-    replay H (txThread b tid rv e0 L e) H' (txThread b' tid rv e0 L' e') ->
-    AheadOf H (Single(txThread b tid rv e0 L e)) (Single(txThread b' tid rv e0 L' e'))
+| aheadOfTXRO : forall tid rv e0 L L' e e',
+    replay H (txThread false tid rv e0 L e) H (txThread false tid rv e0 L' e') ->
+    AheadOf H (Single(txThread false tid rv e0 L e)) (Single(txThread false tid rv e0 L' e'))
+| aheadOfTXRW : forall tid rv b e0 L e,
+    AheadOf H (Single(txThread b tid rv e0 L e)) (Single(txThread b tid rv e0 L e))
 | replayPar : forall T1 T2 T1' T2',
     AheadOf H T1 T1' -> AheadOf H T2 T2' ->
     AheadOf H (Par T1 T2) (Par T1' T2'). 
@@ -132,49 +50,86 @@ Ltac sameStep :=
    eapply decomposeDeterministic in H; eauto; invertHyp; repeat invertEq
   end. 
 
+Theorem logMonotonic : forall H H' tid rv e0 L e L' e',
+    replay H (txThread true tid rv e0 L e) H' (txThread false tid rv e0 L' e') -> False.
+Proof.
+  intros. dependent induction H0.
+  {dependent destruction H0; eauto. }
+Qed. 
+
+
+Theorem AheadOfNI : forall C C' H H' T1 T1' T2 T2',
+    f_step C H T1 C' H' T1' -> AheadOf H T2 T2' ->
+    AheadOf H' T2 T2'.
+Proof.
+  intros. genDeps{{C; T1; C'; T1'}}. 
+  induction H1; intros.
+  {constructor. }
+  {dependent destruction H1.
+   {
+Admitted. 
+    
+                        
 (*partial abort can simulate full abort*)
 Theorem fullImpliesPartial : forall C H T C' H' T' PT, 
                                f_step C H T C' H' T' -> AheadOf H T PT ->
-                               poolRewind C H PT -> 
+                               poolRewind C H PT -> poolRewind C H T ->
                                exists PT', p_multistep C H PT C' H' PT' /\
                                            AheadOf H' T' PT'.
 Proof.
   intros. generalize dependent PT. induction H0; intros. 
   {(*lifted step (full abort)*)
-    inv H0. dependent destruction H1. admit. }
+    inv H0. dependent destruction H3. dependent destruction H4. 
+    {copy H0. eapply validateRewindHeapEq in H6; eauto. simpl in *.
+     subst. eapply replayInvalid in H5; eauto.    
+     assert(rewind H'0 (txThread false tid S e0 NilLog e0) H (txThread false tid S e0 L'0 e'0)).
+     rewrite <- rewindIFFReplay in H4. eapply rewindTrans; eassumption.
+     eapply abortRewind in H6; eauto; try omega. copy H5. 
+     eapply validateValidate in H5. invertHyp. econstructor. split.
+     eapply c_multi_step. eapply c_liftedStep. econstructor. eauto. 
+     constructor. econstructor. rewrite <- rewindIFFReplay. assumption. }
+    {copy H0. eapply validateRewindHeapEq in H4; eauto. simpl in *. subst. 
+     econstructor. split. eapply c_multi_step. eapply c_liftedStep.
+     econstructor; eauto. constructor. econstructor.
+     eapply abortRewind in H5; eauto; try omega. rewrite <- rewindIFFReplay. 
+     assumption. }
+  }
   {(*transactional step*)
     dependent destruction H0.
     {(*checkpoint read*)
-      dependent destruction H3. dependent destruction H4.
-      dependent destruction H3.
-      {econstructor. split. eapply c_multi_step.
-       eapply c_transStep. econstructor; eauto. constructor.
-       econstructor. constructor. }
-      {dependent destruction H4; sameStep. 
-       {transEq. invertEq. econstructor. split. constructor.
-        econstructor. eauto. }
-       {transEq. invertEq. exfalso. eapply validInvalidStamp; eauto. }
+      dependent destruction H3. dependent destruction H6.
+      {dependent destruction H6.
+       {econstructor. split. eapply c_multi_step.
+        eapply c_transStep. econstructor; eauto. constructor.
+        econstructor. constructor. }
+       {dependent destruction H7; sameStep. 
+        {transEq. invertEq. econstructor. split. constructor.
+         econstructor. eauto. }
+        {transEq. invertEq. exfalso. eapply validInvalidStamp; eauto. }
+       }
       }
+      {econstructor. split. eapply c_multi_step.
+        eapply c_transStep. econstructor; eauto. constructor.
+        econstructor. constructor. }
     }
     {(*non-checkpoint read*)
-      dependent destruction H3. dependent destruction H4.
-      dependent destruction H3.
+      dependent destruction H3. dependent destruction H6.
       {econstructor. split. eapply c_multi_step.
        eapply c_transStep. econstructor; eauto. constructor.
-       econstructor. constructor. }
-      {dependent destruction H4; sameStep. 
-       {transEq. invertEq. econstructor. split. constructor.
-        econstructor. eauto. }
-       {transEq. invertEq. exfalso. eapply validInvalidStamp; eauto. }
-      }
+       econstructor. }
     }
     {(*write*)
-      dependent destruction H3. dependent destruction H4.
-      dependent destruction H3.
+      dependent destruction H3. dependent destruction H6.
+      {dependent destruction H6.
+       {econstructor. split. eapply c_multi_step.
+        eapply c_transStep. eapply t_writeLocked; eauto.
+        constructor. econstructor. }
+       {dependent destruction H7; sameStep. exfalso.
+        eapply logMonotonic; eauto. }
+      }
       {econstructor. split. eapply c_multi_step.
-       eapply c_transStep. econstructor; eauto. constructor.
-       econstructor. constructor. }
-      {dependent destruction H4; sameStep. econstructor. admit. }
+        eapply c_transStep. eapply t_writeLocked; eauto.
+        constructor. econstructor. }
     }
     {dependent destruction H1. dependent destruction H2.
      dependent destruction H1.
@@ -183,6 +138,9 @@ Proof.
       constructor. econstructor. constructor. }
      {dependent destruction H1; sameStep. econstructor.
       split. constructor. econstructor. eauto. }
+     {econstructor. split. eapply c_multi_step.
+      eapply c_transStep. eapply t_atomicIdemStep; eauto.
+      constructor. econstructor. }
     }
     {dependent destruction H1. dependent destruction H2.
      dependent destruction H1.
@@ -191,25 +149,28 @@ Proof.
       constructor. econstructor. constructor. }
      {dependent destruction H1; sameStep. econstructor.
       split. constructor. econstructor. eauto. }
+     {econstructor. split. eapply c_multi_step.
+      eapply c_transStep. eapply t_betaStep; eauto.
+      constructor. econstructor. }
     }
   }
-  {inv H1. dependent destruction H2. eapply IHc_step in H5; eauto.
+  {inv H1. dependent destruction H2. inv H3. eapply IHc_step in H6; eauto.
    invertHyp. econstructor. split. eapply multi_L. eauto.
-   econstructor; eauto. admit. (*we need another noninterference lemma for replay*)
-  }
-  {inv H1. dependent destruction H2. eapply IHc_step in H7; eauto.
+   econstructor; eauto.
+
+   eapply AheadOfNI; eauto. }
+  {inv H1. inv H2. inv H3. eapply IHc_step in H8; eauto.
    invertHyp. econstructor. split. eapply multi_R. eauto.
-   econstructor; eauto. admit. (*we need another noninterference lemma for replay*)
-  }
+   econstructor; eauto. eapply AheadOfNI; eauto. }
   {inv H1. inv H2. econstructor. split. eapply c_multi_step.
    eapply c_forkStep; eauto. constructor. repeat constructor. }
   {inv H2. inv H3. econstructor. split. eapply c_multi_step.
    eapply c_allocStep; eauto. constructor. constructor. }
   {dependent destruction H2. dependent destruction H3.
-   dependent destruction H2.
+   dependent destruction H6. dependent destruction H5.
    {econstructor. split. eapply c_multi_step. eapply c_commitStep; eauto.
     constructor. constructor. }
-   {dependent destruction H2; sameStep. }
+   {dependent destruction H5; sameStep. }
   }
   {inv H1. inv H2. econstructor. split. eapply c_multi_step.
    eapply c_atomicStep; eauto. constructor. econstructor. 
