validateWrite.v
@@ -80,24 +80,24 @@ Proof.
   induction H4; intros; try solve[inv Heqv0]. 
   {inv Heqv0. invertHyp. eapply validateNotIn in H5; eauto. 
    invertHyp. heapUnfold. destruct (Nat.eq_dec l0 l).
-   {subst. invertEq. inv H3; inv H1; exfalso; auto. }
+   {subst. invertEq. inv H1; exfalso; auto. }
    {econstructor; eauto. }
   }
   {inv Heqv0. invertHyp. eapply validateNotIn in H5; eauto. 
    invertHyp. heapUnfold. destruct (Nat.eq_dec l0 l).
-   {subst. invertEq. inv H3; inv H1; exfalso; auto. }
+   {subst. invertEq. inv H1; exfalso; auto. }
    {econstructor; eauto. }
   }
   {invertEq. dependent destruction H0.
    {invertHyp. eapply IHvalidate in H1; eauto.
-    subst. eapply readPropAbort; eauto. constructor. }
+    subst. eapply readPropAbort; eauto. constructor. constructor. }
    {invertHyp. eapply IHvalidate in H1; eauto.
-    eapply readPropAbort; eauto. constructor. }
+    eapply readPropAbort; eauto. constructor. constructor. }
   } 
   {invertHyp. invertEq. eapply IHvalidate in H9; eauto.
    heapUnfold. destruct (Nat.eq_dec l0 l). contradiction.
    rewrite updatecomm; auto. eapply writePropAbort. auto.
-   eauto. auto. auto. }
+   eauto. auto. auto. constructor. }
 Qed.
 
 Theorem abortIn :  
@@ -138,4 +138,164 @@ Proof.
    heapUnfold. destruct (Nat.eq_dec l l). invertEq.
    eapply abortNotIn in H2; eauto. constructor. auto. constructor. 
    exfalso; auto. }
+Qed. 
+
+Theorem validateNotInRev : 
+  forall tid l v b v'' lock''' rv wv e0 L H lock' chkpnt HI HV,
+    Log.notIn l b L -> H l = Some(v'', lock''') -> 
+    @validate tid rv wv e0 b L H (commit chkpnt HI HV) -> locked tid lock' ->
+    exists HV', @validate tid rv wv e0 b L (update H l v lock') (commit chkpnt (update HI l v lock') HV'). 
+Proof.
+  intros. remember (commit chkpnt HI HV).
+  genDeps{{chkpnt; HI; HV; l; lock'''; v''; lock'}}. 
+  induction H2; intros; inv Heqv0. 
+  {repeat econstructor. }
+  {invertHyp. eapply IHvalidate in H4; eauto. invertHyp.
+   destruct (Nat.eq_dec l l0). 
+   {subst. econstructor. econstructor. heapUnfold. simplEq l0 l0.
+    auto. Focus 2. eauto. inv H3. constructor. constructor. }
+   {econstructor. econstructor. heapUnfold. simplEq l0 l. eauto.
+    auto. eauto. } constructor. 
+  }
+  {invertHyp. eapply IHvalidate in H4; eauto. invertHyp.
+   destruct (Nat.eq_dec l l0).
+   {subst. econstructor. econstructor. heapUnfold. simplEq l0 l0.
+    auto. Focus 2. eauto. inv H3. constructor. constructor. }
+   {econstructor. econstructor. heapUnfold. simplEq l0 l. eauto.
+    auto. eauto. } constructor. 
+  }
+  {invertHyp. eapply IHvalidate in H5; eauto. invertHyp.
+   econstructor. rewrite updatecomm; auto. econstructor. heapUnfold.
+   simplEq l0 l. eauto. auto. auto. eauto. constructor. }
+Qed. 
+
+Theorem validateInRev :  
+  forall tid l v v'' rv wv e0 L H lock' chkpnt HI HV,
+    Log.In l L -> H l = Some(v'', lock') -> 
+    @validate tid rv wv e0 true L H (commit chkpnt HI HV) ->
+    locked tid lock' ->
+    exists HV', @validate tid rv wv e0 true L (update H l v lock') 
+                     (commit chkpnt HI HV').
+Proof.
+  intros. genDeps{{v''; lock'; v}}. dependent induction H2; intros.
+  {dependent destruction H0. eapply IHvalidate in H0; eauto.
+   invertHyp. destruct (Nat.eq_dec l l0).
+   {econstructor. econstructor. heapUnfold. subst. destruct (Nat.eq_dec l0 l0).
+    auto. exfalso; auto. subst. transEq.
+    invertEq. assumption. eauto. }
+   {econstructor. econstructor; eauto. heapUnfold. simplEq l l0. eauto. }
+  }
+  {dependent destruction H0.
+   {inv H4. transEq. invertEq. eapply validateNotInRev in H0.
+    invertHyp. econstructor.
+    replace (commit chkpnt (update HI0 l0 v1 (Unlocked oldV0)) ?HV') with
+    (commit chkpnt (update (update HI0 l0 v0 (Locked tid oldV0 v1)) l0 v1 (Unlocked oldV0)) ?HV'). 
+    Focus 2. rewrite updateUpdate. eauto. econstructor. heapUnfold. simplEq l0 l0.
+    auto. eauto. eauto. eauto. eauto. eauto. constructor. }
+   {eapply IHvalidate in H4; eauto. invertHyp. econstructor.
+    econstructor; eauto. heapUnfold. simplEq l l0. eauto. }
+  }
+Qed. 
+
+Theorem validateNotInLookup : forall b tid rv wv e0 L H res l,
+    @validate tid rv wv e0 b L H res -> Log.notIn l b L ->
+    H l = (invalidHeap res) l. 
+Proof.
+  intros. induction H0; try solve[simpl in *; dependent destruction H1; eauto]. 
+  {simpl in *. dependent destruction H1. unfold update. simplEq l0 l. 
+   auto. }
+  {dependent destruction H2. invertHyp. eauto. 
+   invertHyp. eauto. }
+  {simpl in *. invertHyp. unfold update.
+   simplEq l0 l. auto. }
+Qed. 
+
+Theorem validateAcquiredLockRev : forall tid l v v' b rv wv e0 L L' H lock lock' chkpnt HI HV,
+    H l = Some(v', lock) ->
+    acquireLock l v' tid rv L lock lock' L' ->
+    @validate tid rv wv e0 b L H (commit chkpnt HI HV) ->
+    exists HV', @validate tid rv wv e0 true L' (update H l v lock') (commit chkpnt HI HV'). 
+Proof.
+  intros. dependent destruction H1. 
+  {eapply validateInRev in H2; eauto. constructor. }
+  {copy H3. eapply validateNotInRev in H3; eauto. invertHyp. Focus 2. constructor. auto.
+   replace HI with (update (update HI l v (Locked tid S' v')) l v' (Unlocked S')). econstructor.
+   econstructor. heapUnfold. simplEq l l. reflexivity. eauto.
+   auto. eauto. rewrite updateUpdate. eapply updateIdempotent.
+   eapply validateNotInLookup in H4; eauto.
+   simpl in *. rewrite <- H4. assumption. }
+Qed.
+
+
+Theorem abortNotInRev : 
+  forall tid l v b v'' lock''' rv wv e0 L H lock' chkpnt HI,
+    Log.notIn l b L -> H l = Some(v'', lock''') -> 
+    @validate tid rv wv e0 b L H (abort chkpnt HI) -> locked tid lock' ->
+    validStamp tid rv lock''' ->
+    @validate tid rv wv e0 b L (update H l v lock') (abort chkpnt (update HI l v lock')). 
+Proof.
+  intros. remember (abort chkpnt HI).
+  genDeps{{chkpnt; HI; l; v; v''; lock'''; lock'}}.
+  induction H2; intros; inv Heqv0.  
+  {invertHyp. destruct (Nat.eq_dec l l0).
+   {subst. exfalso. eapply validInvalidStamp; eauto. 
+    transEq. invertEq. assumption. }
+   {eapply validateNotInRev in H2; eauto. invertHyp.
+    econstructor; eauto. heapUnfold. simplEq l0 l. eauto. constructor. }
+  }
+  {dependent destruction H5. destruct (Nat.eq_dec l l0).
+   {subst. exfalso. eapply validInvalidStamp; eauto. 
+    transEq. invertEq. assumption. }
+   {eapply validateNotInRev in H2; eauto. invertHyp.
+    econstructor; eauto. heapUnfold. simplEq l0 l. eauto. }
+  }
+  {eapply readPropAbort. eapply IHvalidate; eauto. 
+   dependent destruction H0; invertHyp; auto. auto. }
+  {invertHyp. rewrite updatecomm; auto. eapply writePropAbort; eauto.
+   eapply IHvalidate; eauto. constructor. heapUnfold.
+   simplEq l0 l. eauto. }
+Qed.    
+
+Theorem abortInRev :  
+  forall tid l v v'' rv wv e0 L H lock' chkpnt HI,
+    Log.In l L -> H l = Some(v'', lock') -> 
+    @validate tid rv wv e0 true L H (abort chkpnt HI) ->
+    locked tid lock' ->
+    @validate tid rv wv e0 true L (update H l v lock') 
+              (abort chkpnt HI).
+Proof.
+  intros. genDeps{{v; v''; lock'; l}}. dependent induction H2; intros.
+  {invertHyp. destruct (Nat.eq_dec l l0).
+   {subst. transEq. invertEq. invertHyp. exfalso; auto. }
+   {eapply validateInRev in H2; eauto. invertHyp. econstructor; eauto.
+    heapUnfold. simplEq l0 l. eauto. constructor. }
+  }
+  {eapply readPropAbort; eauto. eapply IHvalidate; eauto.
+   dependent destruction H0; invertHyp; auto. }
+  {invertHyp.
+   {transEq. invertEq.
+    replace (update HI0 l v1 (Unlocked oldV0)) with
+    (update (update HI0 l v0 (Locked tid oldV0 v1)) l v1 (Unlocked oldV0)).
+    eapply writePropAbort. eapply abortNotInRev; eauto. constructor.
+    constructor. heapUnfold. simplEq l l. auto. auto. auto.
+    rewrite updateUpdate. auto. }
+   {eapply writePropAbort. eapply IHvalidate; eauto. constructor.
+    heapUnfold. simplEq l0 l. eauto. auto. auto. }
+  }
+Qed. 
+    
+Theorem abortAcquiredLockRev : forall tid l v v' b rv wv e0 L L' H lock lock' chkpnt HI,
+    H l = Some(v', lock) ->
+    acquireLock l v' tid rv L lock lock' L' ->
+    @validate tid rv wv e0 b L H (abort chkpnt HI) ->
+    @validate tid rv wv e0 true L' (update H l v lock') (abort chkpnt HI). 
+Proof.
+  intros. dependent destruction H1.
+  {eapply abortInRev in H2; eauto. constructor. }
+  {copy H3. eapply abortNotInRev in H3; eauto. 
+   replace HI with (update(update HI l v (Locked tid S' v')) l v' (Unlocked S')).  
+   Focus 2. rewrite updateUpdate. apply updateIdempotent.
+   eapply  validateNotInLookup in H4; eauto. simpl in H4. 
+   rewrite <- H4. assumption. eapply writePropAbort. eauto. heapUnfold.
+   simplEq l l. eauto. auto. auto. constructor. constructor. auto. }
 Qed. 
